HybridVerifVecs/nd_funs/cat2funcset_pre.thy
@@ -91,6 +91,14 @@ abbreviation p2ndf :: "'a pred \<Rightarrow> 'a nd_fun" ("(1\<lceil>_\<rceil>)")
 lemma le_p2ndf_iff[simp]:"\<lceil>P\<rceil> \<le> \<lceil>Q\<rceil> = (\<forall>s. P s \<longrightarrow> Q s)"
   by(transfer, auto simp: le_fun_def)
 
+lemma eq_p2ndf_iff:"(\<lceil>P\<rceil> = \<lceil>Q\<rceil>) = (P = Q)"
+proof(safe)
+  assume "\<lceil>P\<rceil> = \<lceil>Q\<rceil>"
+  hence "\<lceil>P\<rceil> \<le> \<lceil>Q\<rceil> \<and> \<lceil>Q\<rceil> \<le> \<lceil>P\<rceil>" by simp
+  then have "(\<forall>s. P s \<longrightarrow> Q s) \<and> (\<forall>s. Q s \<longrightarrow> P s)" by simp
+  thus "P = Q" by auto
+qed
+
 lemma p2ndf_le_eta[simp]:"\<lceil>P\<rceil> \<le> \<eta>\<^sup>\<bullet>"
   by(transfer, simp add: le_fun_def, clarify)
 
@@ -203,6 +211,25 @@ lemma sqrt_le_itself: "1 \<le> x \<Longrightarrow> sqrt x \<le> x"
 
 lemma sqrt_real_nat_le:"sqrt (real n) \<le> real n"
   by (metis (full_types) abs_of_nat le_square of_nat_mono of_nat_mult real_sqrt_abs2 real_sqrt_le_iff)
+
+lemma semiring_factor_left:"a \<cdot> b + a \<cdot> c = a \<cdot> ((b::('a::semiring)) + c)"
+  by(subst Groups.algebra_simps(18), simp)
+
+lemma sin_cos_squared_add3:"(x::('a:: {banach,real_normed_field})) \<cdot> (sin t)\<^sup>2 + x \<cdot> (cos t)\<^sup>2 = x"
+  by(subst semiring_factor_left, subst sin_cos_squared_add, simp)
+
+lemma sin_cos_squared_add4:"(x::('a:: {banach,real_normed_field})) \<cdot> (cos t)\<^sup>2 + x \<cdot> (sin t)\<^sup>2 = x"
+  by(subst semiring_factor_left, subst sin_cos_squared_add2, simp)
+
+lemma [simp]:"((x::real) \<cdot> cos t - y \<cdot> sin t)\<^sup>2 + (x \<cdot> sin t + y \<cdot> cos t)\<^sup>2 = x\<^sup>2 + y\<^sup>2"
+proof-
+  have "(x \<cdot> cos t - y \<cdot> sin t)\<^sup>2 = x\<^sup>2 \<cdot> (cos t)\<^sup>2 + y\<^sup>2 \<cdot> (sin t)\<^sup>2 - 2 \<cdot> (x \<cdot> cos t) \<cdot> (y \<cdot> sin t)"
+    by(simp add: power2_diff power_mult_distrib)
+  also have "(x \<cdot> sin t + y \<cdot> cos t)\<^sup>2 = y\<^sup>2 \<cdot> (cos t)\<^sup>2 + x\<^sup>2 \<cdot> (sin t)\<^sup>2 + 2 \<cdot> (x \<cdot> cos t) \<cdot> (y \<cdot> sin t)"
+    by(simp add: power2_sum power_mult_distrib)
+  ultimately show "(x \<cdot> cos t - y \<cdot> sin t)\<^sup>2 + (x \<cdot> sin t + y \<cdot> cos t)\<^sup>2 = x\<^sup>2 + y\<^sup>2"  
+    by (simp add: Groups.mult_ac(2) Groups.mult_ac(3) right_diff_distrib sin_squared_eq) 
+qed
 
 lemma closed_segment_mvt:
   fixes f :: "real \<Rightarrow> real"
